code/rsapss/Hacl.Spec.Bignum.fst
@@ -5,105 +5,6 @@ module Loops = Lib.LoopCombinators
 
 #reset-options "--z3rlimit 50 --fuel 0 --ifuel 0"
 
-let bn_is_odd #len b =
-  if len > 0 then
-    FStar.UInt64.(Lib.RawIntTypes.u64_to_UInt64 (b.[0] &. u64 1) =^ 1uL)
-  else false
-
-let bn_is_odd_lemma #len b =
-  if len > 0 then begin
-    bn_eval_split_i #len b 1;
-    bn_eval1 (slice b 0 1);
-    assert (bn_v b % 2 == (v b.[0] + pow2 64 * bn_v (slice b 1 len)) % 2);
-    Math.Lemmas.pow2_plus 1 63;
-    Math.Lemmas.modulo_addition_lemma (v b.[0]) 2 (pow2 63 * bn_v (slice b 1 len));
-    assert (bn_v b % 2 == v b.[0] % 2);
-    mod_mask_lemma b.[0] 1ul;
-    assert (v (mod_mask #U64 #SEC 1ul) == v (u64 1)) end
-  else bn_eval0 #len b
-
-
-val bn_mask_lt_f: #len:size_nat -> a:lbignum len -> b:lbignum len -> i:nat{i < len} -> acc:uint64 -> uint64
-let bn_mask_lt_f #len a b i acc =
-  let beq = eq_mask a.[i] b.[i] in
-  let blt = lt_mask a.[i] b.[i] in
-  mask_select beq acc (mask_select blt (ones U64 SEC) (zeros U64 SEC))
-
-let bn_mask_lt_t (len:size_nat) (i:nat{i <= len}) = uint64
-
-let bn_mask_lt #len a b =
-  Loops.repeat_gen len (bn_mask_lt_t len) (bn_mask_lt_f #len a b) (u64 0)
-
-// val bn_mask_lt_aux: len:size_nat -> a:lbignum len -> b:lbignum len -> k:pos{k <= len} -> Lemma
-//   (requires v a.[k - 1] <> v b.[k - 1])
-//   (ensures (if v a.[k - 1] < v b.[k - 1] then eval_ len a k < eval_ len b k else eval_ len a k > eval_ len b k))
-// let bn_mask_lt_aux len a b k =
-//   if v a.[k - 1] < v b.[k - 1] then bn_eval_lt len a b k else bn_eval_lt len b a k
-
-val bn_mask_lt_lemma_step:
-  #len:size_nat -> a:lbignum len -> b:lbignum len -> k:pos{k <= len} -> mask0:uint64 -> Lemma
-  (requires
-    (if v mask0 = 0 then eval_ len a (k - 1) >= eval_ len b (k - 1) else eval_ len a (k - 1) < eval_ len b (k - 1)) /\
-    (v mask0 == 0 \/ v mask0 == v (ones U64 SEC)))
-  (ensures (let mask = bn_mask_lt_f #len a b (k - 1) mask0 in
-    (if v mask = 0 then eval_ len a k >= eval_ len b k else eval_ len a k < eval_ len b k) /\
-    (v mask == 0 \/ v mask == v (ones U64 SEC))))
-
-let bn_mask_lt_lemma_step #len a b k mask0 =
-  let mask = bn_mask_lt_f #len a b (k - 1) mask0 in
-  let ai = a.[k - 1] in
-  let bi = b.[k - 1] in
-  let beq = eq_mask ai bi in
-  assert (if v ai = v bi then v beq == v (ones U64 SEC) else v beq == 0);
-  let blt = lt_mask ai bi in
-  assert (if v ai < v bi then v blt == v (ones U64 SEC) else v blt == 0);
-
-  let res0 = mask_select blt (ones U64 SEC) (zeros U64 SEC) in
-  let mask = mask_select beq mask0 res0 in
-  //assert (mask == bn_mask_lt_f #len a b (k - 1) mask0);
-
-  mask_select_lemma blt (ones U64 SEC) (zeros U64 SEC);
-  mask_select_lemma beq mask0 res0;
-
-  if v beq = 0 then begin
-    assert (v mask = v res0);
-    mask_select_lemma blt (ones U64 SEC) (zeros U64 SEC);
-    //assert (v res0 == (if v blt = 0 then 0 else v (ones U64 SEC)));
-    assert (if v mask = 0 then v ai > v bi else v ai < v bi);
-    if v a.[k - 1] < v b.[k - 1] then bn_eval_lt len a b k else bn_eval_lt len b a k;
-    () end
-  else begin
-    assert (v mask = v mask0);
-    //assert (v beq == v (ones U64 SEC));
-    //assert (if v mask = v mask0 then v ai = v bi else v ai <> v bi);
-    assert (v ai == v bi);
-    bn_eval_unfold_i a k;
-    bn_eval_unfold_i b k;
-    () end
-
-
-val bn_mask_lt_lemma_loop:
-  #len:size_nat -> a:lbignum len -> b:lbignum len -> k:nat{k <= len} -> Lemma
-  (let mask = Loops.repeat_gen k (bn_mask_lt_t len) (bn_mask_lt_f #len a b) (u64 0) in
-   (v mask == 0 \/ v mask == v (ones U64 SEC)) /\
-   (if v mask = 0 then eval_ len a k >= eval_ len b k else eval_ len a k < eval_ len b k))
-
-let rec bn_mask_lt_lemma_loop #len a b k =
-  let mask = Loops.repeat_gen k (bn_mask_lt_t len) (bn_mask_lt_f #len a b) (u64 0) in
-  if k = 0 then begin
-    Loops.eq_repeat_gen0 k (bn_mask_lt_t len) (bn_mask_lt_f #len a b) (u64 0);
-    assert (v mask = 0);
-    bn_eval0 a;
-    bn_eval0 b end
-  else begin
-    let mask0 = Loops.repeat_gen (k - 1) (bn_mask_lt_t len) (bn_mask_lt_f #len a b) (u64 0) in
-    Loops.unfold_repeat_gen k (bn_mask_lt_t len) (bn_mask_lt_f #len a b) (u64 0) (k - 1);
-    bn_mask_lt_lemma_loop #len a b (k - 1);
-    bn_mask_lt_lemma_step #len a b k mask0 end
-
-let bn_mask_lt_lemma #len a b =
-  bn_mask_lt_lemma_loop #len a b len
-
 let bn_add #aLen #bLen a b =
   Hacl.Spec.Bignum.Addition.bn_add a b
 
@@ -203,15 +104,8 @@ let bn_sub_mask_lemma #len n a =
 
   Classical.move_requires_2 (bn_eval_inj len) n a
 
-let bn_is_less #len a b =
-  let mask = bn_mask_lt a b in
-  not (FStar.UInt64.(Lib.RawIntTypes.u64_to_UInt64 mask =^ 0uL))
+(* get and set i-th bit of a bignum *)
 
-let bn_is_less_lemma #len a b =
-  bn_mask_lt_lemma #len a b
-
-
-[@CInline]
 let bn_is_bit_set #len input ind =
   let i = ind / 64 in
   let j = ind % 64 in
@@ -247,7 +141,7 @@ let bn_is_bit_set_lemma #len b ind =
   };
   assert (v tmp2 == bn_v b / pow2 ind % 2)
 
-[@CInline]
+
 let bn_bit_set #len input ind =
   let i = ind / 64 in
   let j = ind % 64 in
@@ -266,23 +160,41 @@ let bn_bit_set_lemma_aux a b c d =
   Math.Lemmas.small_division_lemma_1 a (pow2 c)
 
 
+val bn_lt_pow2_index_lemma: #len:size_nat -> b:lbignum len -> ind:size_nat{ind / 64 < len} -> Lemma
+  (requires bn_v b < pow2 ind)
+  (ensures (let i = ind / 64 in v b.[ind / 64] < pow2 (ind % 64) /\
+    bn_v b == bn_v (slice b 0 i) + pow2 (i * 64) * v b.[i] /\
+    bn_v (slice b (i + 1) len) = 0))
+
+let bn_lt_pow2_index_lemma #len b ind =
+  let i = ind / 64 in
+  let j = ind % 64 in
+
+  Math.Lemmas.euclidean_division_definition ind 64;
+  assert (bn_v b < pow2 (i * 64 + j));
+  Math.Lemmas.pow2_lt_compat (i * 64 + 64) (i * 64 + j);
+  assert (bn_v b < pow2 (i * 64 + 64));
+
+  bn_eval_split_i #len b (i + 1);
+  //assert (bn_v b == bn_v (slice b 0 (i + 1)) + pow2 (64 * (i + 1)) * bn_v (slice b (i + 1) len));
+  bn_eval_bound (slice b 0 (i + 1)) (i + 1);
+  //assert (bn_v (slice b 0 (i + 1)) < pow2 (64 * i + 64));
+  bn_bit_set_lemma_aux (bn_v (slice b 0 (i + 1))) (bn_v (slice b (i + 1) len)) (64 * (i + 1)) 0;
+  assert (bn_v b == bn_v (slice b 0 (i + 1)));
+
+  bn_eval_split_i #(i + 1) (slice b 0 (i + 1)) i;
+  //assert (bn_v b == bn_v (slice b 0 i) + pow2 (i * 64) * bn_v (slice b i (i + 1)));
+  bn_eval1 (slice b i (i + 1));
+  assert (bn_v b == bn_v (slice b 0 i) + pow2 (i * 64) * v b.[i]);
+  bn_eval_bound #i (slice b 0 i) i;
+  bn_bit_set_lemma_aux (bn_v (slice b 0 i)) (v b.[i]) (i * 64) j;
+  assert (v b.[i] < pow2 j)
+
+
 let bn_bit_set_lemma #len input ind =
   let i = ind / 64 in
   let j = ind % 64 in
-  Math.Lemmas.euclidean_division_definition ind 64;
-  assert (bn_v input < pow2 (i * 64 + j));
-  Math.Lemmas.pow2_lt_compat (i * 64 + 64) (i * 64 + j);
-  bn_eval_split_i #len input (i + 1);
-  assert (bn_v input == bn_v (slice input 0 (i + 1)));
-  bn_eval_split_i #(i + 1) (slice input 0 (i + 1)) i;
-  //Seq.Properties.slice_slice input 0 (i + 1) 0 i;
-  //Seq.Properties.slice_slice input 0 (i + 1) i (i + 1);
-  assert (bn_v input == bn_v (slice input 0 i) + pow2 (i * 64) * bn_v (slice input i (i + 1)));
-  bn_eval_unfold_i #1 (slice input i (i + 1)) 1;
-  bn_eval0 #1 (slice input i (i + 1));
-  assert (bn_v input == bn_v (slice input 0 i) + pow2 (i * 64) * v input.[i]);
-  bn_eval_bound #i (slice input 0 i) i;
-  bn_bit_set_lemma_aux (bn_v (slice input 0 i)) (v input.[i]) (i * 64) j;
+  bn_lt_pow2_index_lemma #len input ind;
   assert (v input.[i] < pow2 j);
 
   let b = u64 1 <<. size j in
@@ -295,11 +207,12 @@ let bn_bit_set_lemma #len input ind =
 
   calc (==) {
     bn_v inp;
-    (==) { bn_eval_split_i #len inp (i + 1) }
+    (==) { bn_eval_split_i #len inp (i + 1);
+    bn_eval_extensionality_j (slice inp (i + 1) len) (slice input (i + 1) len) (len - i - 1) }
     bn_v (slice inp 0 (i + 1));
     (==) { bn_eval_split_i #(i + 1) (slice inp 0 (i + 1)) i }
     bn_v (slice inp 0 i) + pow2 (i * 64) * bn_v (slice inp i (i + 1));
-    (==) { bn_eval_unfold_i #1 (slice inp i (i + 1)) 1; bn_eval0 #1 (slice inp i (i + 1)) }
+    (==) { bn_eval1 (slice inp i (i + 1)) }
     bn_v (slice inp 0 i) + pow2 (i * 64) * v inp.[i];
     (==) { bn_eval_extensionality_j input inp i }
     bn_v (slice input 0 i) + pow2 (i * 64) * v inp.[i];
@@ -313,6 +226,179 @@ let bn_bit_set_lemma #len input ind =
     bn_v input + pow2 ind;
   }
 
+
+(* Bignum comparison and test functions *)
+
+let bn_is_zero #len b =
+  let bn_zero = create len (u64 0) in
+  let mask = Lib.ByteSequence.seq_eq_mask b bn_zero len in
+  FStar.UInt64.(Lib.RawIntTypes.u64_to_UInt64 mask =^ ones U64 PUB)
+
+let bn_is_zero_lemma #len b =
+  let bn_zero = create len (u64 0) in
+  bn_eval_zeroes len len;
+  let mask = Lib.ByteSequence.seq_eq_mask b bn_zero len in
+  assert (b == bn_zero ==> v mask == v (ones U64 SEC));
+  assert (b =!= bn_zero ==> v mask == v (zeros U64 SEC));
+  Classical.move_requires_2 (bn_eval_inj len) b bn_zero;
+  assert (bn_is_zero #len b == (if bn_v b = bn_v bn_zero then true else false))
+
+
+let bn_is_odd #len b =
+  if len > 0 then
+    FStar.UInt64.(Lib.RawIntTypes.u64_to_UInt64 (b.[0] &. u64 1) =^ 1uL)
+  else false
+
+let bn_is_odd_lemma #len b =
+  if len > 0 then begin
+    bn_eval_split_i #len b 1;
+    bn_eval1 (slice b 0 1);
+    assert (bn_v b % 2 == (v b.[0] + pow2 64 * bn_v (slice b 1 len)) % 2);
+    Math.Lemmas.pow2_plus 1 63;
+    Math.Lemmas.modulo_addition_lemma (v b.[0]) 2 (pow2 63 * bn_v (slice b 1 len));
+    assert (bn_v b % 2 == v b.[0] % 2);
+    mod_mask_lemma b.[0] 1ul;
+    assert (v (mod_mask #U64 #SEC 1ul) == v (u64 1)) end
+  else bn_eval0 #len b
+
+
+val bn_mask_lt_f: #len:size_nat -> a:lbignum len -> b:lbignum len -> i:nat{i < len} -> acc:uint64 -> uint64
+let bn_mask_lt_f #len a b i acc =
+  let beq = eq_mask a.[i] b.[i] in
+  let blt = lt_mask a.[i] b.[i] in
+  mask_select beq acc (mask_select blt (ones U64 SEC) (zeros U64 SEC))
+
+let bn_mask_lt_t (len:size_nat) (i:nat{i <= len}) = uint64
+
+let bn_mask_lt #len a b =
+  Loops.repeat_gen len (bn_mask_lt_t len) (bn_mask_lt_f #len a b) (u64 0)
+
+// val bn_mask_lt_aux: len:size_nat -> a:lbignum len -> b:lbignum len -> k:pos{k <= len} -> Lemma
+//   (requires v a.[k - 1] <> v b.[k - 1])
+//   (ensures (if v a.[k - 1] < v b.[k - 1] then eval_ len a k < eval_ len b k else eval_ len a k > eval_ len b k))
+// let bn_mask_lt_aux len a b k =
+//   if v a.[k - 1] < v b.[k - 1] then bn_eval_lt len a b k else bn_eval_lt len b a k
+
+val bn_mask_lt_lemma_step:
+  #len:size_nat -> a:lbignum len -> b:lbignum len -> k:pos{k <= len} -> mask0:uint64 -> Lemma
+  (requires
+    (if v mask0 = 0 then eval_ len a (k - 1) >= eval_ len b (k - 1) else eval_ len a (k - 1) < eval_ len b (k - 1)) /\
+    (v mask0 == 0 \/ v mask0 == v (ones U64 SEC)))
+  (ensures (let mask = bn_mask_lt_f #len a b (k - 1) mask0 in
+    (if v mask = 0 then eval_ len a k >= eval_ len b k else eval_ len a k < eval_ len b k) /\
+    (v mask == 0 \/ v mask == v (ones U64 SEC))))
+
+let bn_mask_lt_lemma_step #len a b k mask0 =
+  let mask = bn_mask_lt_f #len a b (k - 1) mask0 in
+  let ai = a.[k - 1] in
+  let bi = b.[k - 1] in
+  let beq = eq_mask ai bi in
+  assert (if v ai = v bi then v beq == v (ones U64 SEC) else v beq == 0);
+  let blt = lt_mask ai bi in
+  assert (if v ai < v bi then v blt == v (ones U64 SEC) else v blt == 0);
+
+  let res0 = mask_select blt (ones U64 SEC) (zeros U64 SEC) in
+  let mask = mask_select beq mask0 res0 in
+  //assert (mask == bn_mask_lt_f #len a b (k - 1) mask0);
+
+  mask_select_lemma blt (ones U64 SEC) (zeros U64 SEC);
+  mask_select_lemma beq mask0 res0;
+
+  if v beq = 0 then begin
+    assert (v mask = v res0);
+    mask_select_lemma blt (ones U64 SEC) (zeros U64 SEC);
+    //assert (v res0 == (if v blt = 0 then 0 else v (ones U64 SEC)));
+    assert (if v mask = 0 then v ai > v bi else v ai < v bi);
+    if v a.[k - 1] < v b.[k - 1] then bn_eval_lt len a b k else bn_eval_lt len b a k;
+    () end
+  else begin
+    assert (v mask = v mask0);
+    //assert (v beq == v (ones U64 SEC));
+    //assert (if v mask = v mask0 then v ai = v bi else v ai <> v bi);
+    assert (v ai == v bi);
+    bn_eval_unfold_i a k;
+    bn_eval_unfold_i b k;
+    () end
+
+
+val bn_mask_lt_lemma_loop:
+  #len:size_nat -> a:lbignum len -> b:lbignum len -> k:nat{k <= len} -> Lemma
+  (let mask = Loops.repeat_gen k (bn_mask_lt_t len) (bn_mask_lt_f #len a b) (u64 0) in
+   (v mask == 0 \/ v mask == v (ones U64 SEC)) /\
+   (if v mask = 0 then eval_ len a k >= eval_ len b k else eval_ len a k < eval_ len b k))
+
+let rec bn_mask_lt_lemma_loop #len a b k =
+  let mask = Loops.repeat_gen k (bn_mask_lt_t len) (bn_mask_lt_f #len a b) (u64 0) in
+  if k = 0 then begin
+    Loops.eq_repeat_gen0 k (bn_mask_lt_t len) (bn_mask_lt_f #len a b) (u64 0);
+    assert (v mask = 0);
+    bn_eval0 a;
+    bn_eval0 b end
+  else begin
+    let mask0 = Loops.repeat_gen (k - 1) (bn_mask_lt_t len) (bn_mask_lt_f #len a b) (u64 0) in
+    Loops.unfold_repeat_gen k (bn_mask_lt_t len) (bn_mask_lt_f #len a b) (u64 0) (k - 1);
+    bn_mask_lt_lemma_loop #len a b (k - 1);
+    bn_mask_lt_lemma_step #len a b k mask0 end
+
+let bn_mask_lt_lemma #len a b =
+  bn_mask_lt_lemma_loop #len a b len
+
+
+let bn_is_less #len a b =
+  let mask = bn_mask_lt a b in
+  FStar.UInt64.(Lib.RawIntTypes.u64_to_UInt64 mask =^ ones U64 PUB)
+
+let bn_is_less_lemma #len a b =
+  bn_mask_lt_lemma #len a b
+
+// we could compare bBits with x, but we don't have the bn_num_bits function
+// bn_v b < pow2 x
+let bn_lt_pow2 #len b x =
+  if x >= 64 * len then true
+  else begin
+    let b2 = create len (u64 0) in
+    let b2 = bn_bit_set b2 x in
+    bn_is_less b b2 end
+
+let bn_lt_pow2_lemma #len b x =
+  bn_eval_bound #len b len;
+  assert (bn_v b < pow2 (64 * len));
+  if x >= 64 * len then
+    Math.Lemmas.pow2_le_compat x (64 * len)
+  else begin
+    let b2 = create len (u64 0) in
+    bn_eval_zeroes len len;
+    assert (bn_v b2 = 0);
+    //assert (bn_v b2 < pow2 x);
+    let b2' = bn_bit_set b2 x in
+    bn_bit_set_lemma b2 x;
+    assert (bn_v b2' == pow2 x);
+    bn_is_less_lemma b b2' end
+
+//pow2 x < bn_v b
+let bn_gt_pow2 #len b x =
+  if x >= 64 * len then false
+  else begin
+    let b2 = create len (u64 0) in
+    let b2 = bn_bit_set b2 x in
+    bn_is_less b2 b end
+
+let bn_gt_pow2_lemma #len b x =
+  bn_eval_bound #len b len;
+  assert (bn_v b < pow2 (64 * len));
+  if x >= 64 * len then
+    Math.Lemmas.pow2_le_compat x (64 * len)
+  else begin
+    let b2 = create len (u64 0) in
+    bn_eval_zeroes len len;
+    assert (bn_v b2 = 0);
+    //assert (bn_v b2 < pow2 x);
+    let b2' = bn_bit_set b2 x in
+    bn_bit_set_lemma b2 x;
+    assert (bn_v b2' == pow2 x);
+    bn_is_less_lemma b2' b end
+
+(* Conversion functions *)
 
 let bn_from_uint len x =
   let b = create len (u64 0) in
